add 2 methods in deadlockfreedom_automation

RingBuffer/DeadlockFreedom_Automation.thy
@@ -3,9 +3,12 @@
  * This version combines the lemmas in DeadlockFreenessStuff by Benoit and lemmas in Bounded_Buffer_211124_ddf_automation_incomplete by Simon.
  * 03 Feb 2025
 
+ * updated due to DeadlockFreenessStuff.thy update by Benoit
+ * 25 Feb 2025
+
 *******************************************************************\<close>
 theory DeadlockFreedom_Automation
-  imports "HOL-CSP_OpSem.AfterDeadlockResults" Guard
+  imports "HOL-CSP_OpSem.OpSem_Deadlock_Results" "Guard"
 begin
 
 (**)
@@ -14,9 +17,9 @@ lemma prefix_proving_Mndetprefix_ref :
   \<open>A \<subseteq> B \<Longrightarrow> A \<noteq> {} \<Longrightarrow> (\<And>a. a \<in> A \<Longrightarrow> P a \<sqsubseteq>\<^sub>F\<^sub>D Q a) \<Longrightarrow> (\<sqinter>a \<in> B \<rightarrow> P a) \<sqsubseteq>\<^sub>F\<^sub>D (\<sqinter>a \<in> A \<rightarrow> Q a)\<close>
   \<open>A \<subseteq> B \<Longrightarrow> A \<noteq> {} \<Longrightarrow> (\<And>a. a \<in> A \<Longrightarrow> P a \<sqsubseteq>\<^sub>F\<^sub>D Q a) \<Longrightarrow> (\<sqinter>a \<in> B \<rightarrow> P a) \<sqsubseteq>\<^sub>F\<^sub>D (\<box>a \<in> A \<rightarrow> Q a)\<close>
   \<open>a \<in> B \<Longrightarrow> P a \<sqsubseteq>\<^sub>F\<^sub>D R \<Longrightarrow> (\<sqinter>a \<in> B \<rightarrow> P a) \<sqsubseteq>\<^sub>F\<^sub>D a \<rightarrow> R\<close>
-    apply (metis CSP.mono_Mndetprefix_FD mono_Mndetprefix_FD_set trans_FD)
-   apply (metis CSP.mono_Mprefix_FD Mprefix_refines_Mndetprefix_FD mono_Mndetprefix_FD_set trans_FD)
-  by (meson CSP_Laws.mono_write0_FD Mndetprefix_refine_FD failure_divergence_refine_def order_trans)
+  apply (metis Mndetprefix_FD_subset mono_Mndetprefix_FD order_trans)
+  apply (metis Mndetprefix_FD_Mprefix Mndetprefix_FD_subset mono_Mndetprefix_FD order.trans)
+  by (meson Mndetprefix_FD_write0 dual_order.trans mono_write0_FD)
 
 thm Mndetprefix_def
 
@@ -37,8 +40,8 @@ lemma binops_proving_Mndetprefix_ref :
   \<open>(\<sqinter>a \<in> A \<rightarrow> P a) \<sqsubseteq>\<^sub>F\<^sub>D Q \<Longrightarrow> (\<sqinter>a \<in> A \<rightarrow> P a) \<sqsubseteq>\<^sub>F\<^sub>D R \<Longrightarrow> (\<sqinter>a \<in> A \<rightarrow> P a) \<sqsubseteq>\<^sub>F\<^sub>D Q \<sqinter> R\<close>
   \<open>(\<sqinter>a \<in> A \<rightarrow> P a) \<sqsubseteq>\<^sub>F\<^sub>D Q \<Longrightarrow> (\<sqinter>a \<in> A \<rightarrow> P a) \<sqsubseteq>\<^sub>F\<^sub>D R \<Longrightarrow> (\<sqinter>a \<in> A \<rightarrow> P a) \<sqsubseteq>\<^sub>F\<^sub>D Q \<box> R\<close>
   \<open>(\<sqinter>a \<in> A \<rightarrow> P a) \<sqsubseteq>\<^sub>F\<^sub>D Q \<Longrightarrow> (\<sqinter>a \<in> A \<rightarrow> P a) \<sqsubseteq>\<^sub>F\<^sub>D R \<Longrightarrow> (\<sqinter>a \<in> A \<rightarrow> P a) \<sqsubseteq>\<^sub>F\<^sub>D Q \<rhd> R\<close>
-    apply (metis CSP.mono_Ndet_FD Ndet_id)
-   apply (metis CSP.mono_Det_FD Det_id)
+  apply (simp add: FD_iff_eq_Ndet Ndet_assoc)
+  apply (simp add: FD_iff_eq_Ndet Ndet_distrib_Det_left)
   by (metis Sliding_id mono_Sliding_FD)
 
 
@@ -138,6 +141,7 @@ lemma D_iterate_Mndetprefix :
    (if A = {} then if i = 0 then \<D> P else {}
     else {s @ t| s t. set s \<subseteq> ev ` A \<and> length s = i \<and> t \<in> \<D> P})\<close>
   (is \<open>?lhs P i = (if A = {} then if i = 0 then \<D> P else {} else ?rhs P i)\<close>)
+  for P :: \<open>('a, 'r) process\<^sub>p\<^sub>t\<^sub>i\<^sub>c\<^sub>k\<close>
 proof (split if_split, intro conjI impI)
   show \<open>A = {} \<Longrightarrow> ?lhs P i = (if i = 0 then \<D> P else {})\<close>
     by (cases i) (simp_all add: D_STOP)
@@ -152,18 +156,17 @@ next
     also from "*" have \<open>\<dots> = ?rhs (\<sqinter>a \<in> A \<rightarrow> P) i\<close> .
     also have \<open>\<dots> = ?rhs P (Suc i)\<close>
     proof safe
-      fix s t assume \<open>set s \<subseteq> ev ` A\<close> \<open>t \<in> \<D> (\<sqinter>a\<in>A \<rightarrow> P)\<close> \<open>i = length s\<close>
+      fix s t :: \<open>('a, 'r) trace\<^sub>p\<^sub>t\<^sub>i\<^sub>c\<^sub>k\<close> assume \<open>set s \<subseteq> ev ` A\<close> \<open>t \<in> \<D> (\<sqinter>a\<in>A \<rightarrow> P)\<close> \<open>i = length s\<close>
       from \<open>t \<in> \<D> (\<sqinter>a\<in>A \<rightarrow> P)\<close>
       obtain a t' where \<open>a \<in> A\<close> \<open>t = ev a # t'\<close> \<open>t' \<in> \<D> P\<close>
-        by (simp add: D_Mndetprefix write0_def D_Mprefix \<open>A \<noteq> {}\<close>)
-           (metis list.collapse)
+        by (auto simp add: D_Mndetprefix write0_def D_Mprefix \<open>A \<noteq> {}\<close>)
       from this(1, 2) have \<open>s @ t = (s @ [ev a]) @ t'\<close> \<open>set (s @ [ev a]) \<subseteq> ev ` A\<close>
                            \<open>length (s @ [ev a]) = Suc (length s)\<close>
         by (simp_all add: \<open>set s \<subseteq> ev ` A\<close>)
       with \<open>t' \<in> \<D> P\<close> show \<open>\<exists>s' t'. s @ t = s' @ t' \<and> set s' \<subseteq> ev ` A \<and>
                                      length s' = Suc (length s) \<and> t' \<in> \<D> P\<close> by blast
     next
-      fix s t 
+      fix s t :: \<open>('a, 'r) trace\<^sub>p\<^sub>t\<^sub>i\<^sub>c\<^sub>k\<close>
       assume \<open>set s \<subseteq> ev ` A\<close> \<open>length s = Suc i\<close> \<open>t \<in> \<D> P\<close>
       from this(1, 2) obtain a s'
         where \<open>a \<in> A\<close> \<open>s = s' @ [ev a]\<close> \<open>set s' \<subseteq> ev ` A\<close> \<open>length s' = i\<close>
@@ -177,10 +180,11 @@ next
     finally show \<open>?lhs P (Suc i) = ?rhs P (Suc i)\<close> .
   qed
 qed
-      
+
+
 lemma tickFree_iff_set_range_ev : \<open>tickFree s \<longleftrightarrow> set s \<subseteq> range ev\<close>
-  by (metis event.distinct(1) event.exhaust imageE
-            rangeI subset_code(1) tickFree_def)
+  by (metis (no_types, lifting) Hiding_tickFree empty_filter_conv image_mono list.set_map subset_code(1)
+      tickFree_iff_is_map_ev top_greatest)
 
 (*when A = UNIV, the failure set of a process P that iterates i times over Mndetprefix on A*)
 corollary F_iterate_Mndetprefix_UNIV :
@@ -203,22 +207,19 @@ corollary D_iterate_Mndetprefix_UNIV :
 
 (* TODO : find a better name *)
 
-text \<open> York: I've change the notation for the GlobalNdet_iteration operator to use a "+" instead of a "*". This is because   the requirement is that the process can do some number of steps n > 0 before becoming P. This kind of "at least 1"   behaviour is normally given by a "+" rather than "*". 24Jan25\<close>
 
-definition GlobalNdet_iterations :: \<open>'a process \<Rightarrow> 'a process\<close> (\<open>(_\<^sup>p\<^sup>r\<^sup>o\<^sup>c\<^sup>+)\<close> [1000] 999)
+definition GlobalNdet_iterations :: \<open>('a, 'r) process\<^sub>p\<^sub>t\<^sub>i\<^sub>c\<^sub>k \<Rightarrow> ('a, 'r) process\<^sub>p\<^sub>t\<^sub>i\<^sub>c\<^sub>k\<close> (\<open>(_\<^sup>p\<^sup>r\<^sup>o\<^sup>c\<^sup>+)\<close> [1000] 999)
   where \<open>GlobalNdet_iterations P \<equiv> \<sqinter>i \<in> {0<..}. iterate i\<cdot>(\<Lambda> X. \<sqinter>a\<in>UNIV \<rightarrow> X)\<cdot>P\<close>
 (*this extends iterate i indefinitely, allowing P to be prefixed by an arbitrary but finite number (>0) of Mndetprefix, with the number of iterations being Ndet*)
 
 
-text \<open>York:  This new operator, which uses the * syntax, says that we can perform 0 events and then behave as P. These two operators  ought to be linked together with some lemmas. 24Jan25\<close>
+text \<open>This new operator, which uses the * syntax, says that we can perform 0 or more events and then behave as P. These two operators  ought to be linked together with some lemmas. 24Jan25\<close>
 
-definition GlobalNdet_iterations' :: \<open>'a process \<Rightarrow> 'a process\<close> (\<open>(_\<^sup>p\<^sup>r\<^sup>o\<^sup>c\<^sup>*)\<close> [1000] 999)
+definition GlobalNdet_iterations' :: \<open>('a, 'r) process\<^sub>p\<^sub>t\<^sub>i\<^sub>c\<^sub>k \<Rightarrow> ('a, 'r) process\<^sub>p\<^sub>t\<^sub>i\<^sub>c\<^sub>k\<close> (\<open>(_\<^sup>p\<^sup>r\<^sup>o\<^sup>c\<^sup>*)\<close> [1000] 999)
   where \<open>GlobalNdet_iterations' P \<equiv> \<sqinter>i \<in> UNIV. iterate i\<cdot>(\<Lambda> X. \<sqinter>a\<in>UNIV \<rightarrow> X)\<cdot>P\<close>
   (* UNIV = {0..} *)
 
-text \<open>York:  The below is a lemma  P\<^sup>p\<^sup>r\<^sup>o\<^sup>c\<^sup>+ \<sqsubseteq>\<^sub>F \<sqinter>a\<in>UNIV \<rightarrow>  P\<^sup>p\<^sup>r\<^sup>o\<^sup>c* we think should be true, but we can't prove it as yet 4Jan25 \<close>
 
-text\<open>Benoit 30Jan\<close>
 lemma GlobalNdet_iterations'_is_Ndet_GlobalNdet_iterations : \<open>P\<^sup>p\<^sup>r\<^sup>o\<^sup>c\<^sup>* = P \<sqinter> P\<^sup>p\<^sup>r\<^sup>o\<^sup>c\<^sup>+\<close>
 proof -
   have \<open>UNIV = insert (0 :: nat) {0<..}\<close> by fast
@@ -235,56 +236,53 @@ proof -
   finally show \<open>P\<^sup>p\<^sup>r\<^sup>o\<^sup>c\<^sup>* = P \<sqinter> P\<^sup>p\<^sup>r\<^sup>o\<^sup>c\<^sup>+\<close> .
 qed
 
-text\<open>Benoit 30Jan\<close>
-lemma GlobalNdet_iterations'_Mndetprefix :  \<open>(\<sqinter>a\<in>UNIV \<rightarrow>  P)\<^sup>p\<^sup>r\<^sup>o\<^sup>c\<^sup>* = P\<^sup>p\<^sup>r\<^sup>o\<^sup>c\<^sup>+\<close>
+
+lemma GlobalNdet_iterations'_Mndetprefix : \<open>(\<sqinter>a\<in>UNIV \<rightarrow>  P)\<^sup>p\<^sup>r\<^sup>o\<^sup>c\<^sup>* = P\<^sup>p\<^sup>r\<^sup>o\<^sup>c\<^sup>+\<close>
 proof -
   have \<open>(\<sqinter>a\<in>UNIV \<rightarrow>  P)\<^sup>p\<^sup>r\<^sup>o\<^sup>c\<^sup>* = (\<sqinter> i\<in>UNIV. iterate i\<cdot>(\<Lambda> X. \<sqinter>a\<in>UNIV \<rightarrow>  X)\<cdot>(\<sqinter>a\<in>UNIV \<rightarrow>  P))\<close>
     by (simp add: GlobalNdet_iterations'_def)
   also have \<open>\<dots> = \<sqinter> i\<in>UNIV. iterate (Suc i)\<cdot>(\<Lambda> X. \<sqinter>a\<in>UNIV \<rightarrow>  X)\<cdot>P\<close>
     by (rule mono_GlobalNdet_eq) (simp del: iterate_Suc add: iterate_Suc2)
   also have \<open>\<dots> = \<sqinter> i\<in>{0<..}. iterate i\<cdot>(\<Lambda> X. \<sqinter>a\<in>UNIV \<rightarrow>  X)\<cdot>P\<close>
-    by (simp add: inj_on_mapping_over_GlobalNdet[of Suc UNIV, simplified]
-                  greaterThan_0 mono_GlobalNdet_eq)
+    by (auto simp add: inj_on_mapping_over_GlobalNdet[of Suc UNIV, simplified]
+        greaterThan_0 intro: mono_GlobalNdet_eq)
   also have \<open>\<dots> = P\<^sup>p\<^sup>r\<^sup>o\<^sup>c\<^sup>+\<close> by (simp add: GlobalNdet_iterations_def)
   finally show \<open>(\<sqinter>a\<in>UNIV \<rightarrow>  P)\<^sup>p\<^sup>r\<^sup>o\<^sup>c\<^sup>* = P\<^sup>p\<^sup>r\<^sup>o\<^sup>c\<^sup>+\<close> .
 qed
 
-text\<open>Benoit 30Jan, the original lemma is  P\<^sup>p\<^sup>r\<^sup>o\<^sup>c\<^sup>+ \<sqsubseteq>\<^sub>F \<sqinter>a\<in>UNIV \<rightarrow>  P\<^sup>p\<^sup>r\<^sup>o\<^sup>c*\<close>
-lemma GlobalNdet_iterations_is_one_step_ahead_GlobalNdet_iterations' : \<open>P\<^sup>p\<^sup>r\<^sup>o\<^sup>c\<^sup>+ = \<sqinter>a\<in>UNIV \<rightarrow> P\<^sup>p\<^sup>r\<^sup>o\<^sup>c\<^sup>*\<close>
+
+
+lemma GlobalNdet_iterations_is_one_step_ahead_GlobalNdet_iterations' :\<open>P\<^sup>p\<^sup>r\<^sup>o\<^sup>c\<^sup>+ = \<sqinter>a\<in>UNIV \<rightarrow> P\<^sup>p\<^sup>r\<^sup>o\<^sup>c\<^sup>*\<close>
 proof (subst Process_eq_spec, safe)
   show \<open>t \<in> \<D> (P\<^sup>p\<^sup>r\<^sup>o\<^sup>c\<^sup>+) \<Longrightarrow> t \<in> \<D> (\<sqinter>a\<in>UNIV \<rightarrow>  P\<^sup>p\<^sup>r\<^sup>o\<^sup>c\<^sup>*)\<close> for t
     apply (simp add: D_Mndetprefix write0_def D_Mprefix)
     apply (simp add: GlobalNdet_iterations_def GlobalNdet_iterations'_def)
-    apply (cases t, simp_all add:  D_GlobalNdet D_iterate_Mndetprefix_UNIV)
-    by (metis event.exhaust greaterThan_iff hd_append2 length_greater_0_conv
-              list.sel(1, 3) list.set_sel(1) tickFree_def tickFree_tl tl_append_if)
+    apply (cases t, simp_all add:  D_GlobalNdet D_iterate_Mndetprefix_UNIV greaterThan_0)
+    by (metis (no_types, lifting) append_eq_Cons_conv is_ev_def length_greater_0_conv
+              tickFree_Cons_iff zero_less_Suc)
 next
   show \<open>t \<in> \<D> (\<sqinter>a\<in>UNIV \<rightarrow>  P\<^sup>p\<^sup>r\<^sup>o\<^sup>c\<^sup>*) \<Longrightarrow> t \<in> \<D> (P\<^sup>p\<^sup>r\<^sup>o\<^sup>c\<^sup>+)\<close> for t
     apply (simp add: D_Mndetprefix write0_def D_Mprefix)
     apply (simp add: GlobalNdet_iterations_def GlobalNdet_iterations'_def)
-    apply (cases t, simp_all add:  D_GlobalNdet D_iterate_Mndetprefix_UNIV)
-    by (metis append_Cons event.simps(3) greaterThan_iff length_greater_0_conv list.simps(3) tickFree_Cons_iff)
+    apply (cases t, simp_all add: D_GlobalNdet D_iterate_Mndetprefix_UNIV greaterThan_0)
+    by (metis append_Cons event\<^sub>p\<^sub>t\<^sub>i\<^sub>c\<^sub>k.disc(1) length_Cons tickFree_Cons_iff)
 next
   show \<open>(t, X) \<in> \<F> (P\<^sup>p\<^sup>r\<^sup>o\<^sup>c\<^sup>+) \<Longrightarrow> (t, X) \<in> \<F> (\<sqinter>a\<in>UNIV \<rightarrow>  P\<^sup>p\<^sup>r\<^sup>o\<^sup>c\<^sup>*)\<close> for t X
     apply (simp add: F_Mndetprefix write0_def F_Mprefix)
     apply (simp add: GlobalNdet_iterations_def GlobalNdet_iterations'_def)
     apply (simp add: F_GlobalNdet F_iterate_Mndetprefix_UNIV)
-    apply (cases t, simp_all)
-    by (metis bot_nat_0.not_eq_extremum event.exhaust greaterThan_iff hd_append2 less_iff_Suc_add
-              list.sel(1, 3) list.set_sel(1) list.size(3) tickFree_def tickFree_tl tl_append_if)
+    apply (cases t, simp_all add: greaterThan_0 append_eq_Cons_conv is_ev_def)
+    by (smt (verit, best) append_eq_Cons_conv is_ev_def length_greater_0_conv
+            tickFree_Cons_iff zero_less_Suc)
 next
   show \<open>(t, X) \<in> \<F> (\<sqinter>a\<in>UNIV \<rightarrow>  P\<^sup>p\<^sup>r\<^sup>o\<^sup>c\<^sup>*) \<Longrightarrow> (t, X) \<in> \<F> (P\<^sup>p\<^sup>r\<^sup>o\<^sup>c\<^sup>+)\<close> for t X
     apply (simp add: F_Mndetprefix write0_def F_Mprefix)
     apply (simp add: GlobalNdet_iterations_def GlobalNdet_iterations'_def)
     apply (simp add: F_GlobalNdet F_iterate_Mndetprefix_UNIV)
-    apply (cases t, simp_all add: gt_ex)
-    by (metis append_Cons event.simps(3) greaterThan_0 length_Cons lessI range_eqI tickFree_Cons_iff)
+    apply (cases t, simp_all add: gt_ex greaterThan_0)
+    by (meson Cons_eq_appendI event\<^sub>p\<^sub>t\<^sub>i\<^sub>c\<^sub>k.disc(1) length_Suc_conv tickFree_Cons_iff)
 qed
 
-
-
-
-text \<open> York: This would allow us to prove the following lemma:24Jan25 \<close>
 
 text\<open>Benoit 30Jan, changed from \<open>\<sqinter>a\<in>UNIV \<rightarrow> P\<^sup>p\<^sup>r\<^sup>o\<^sup>c*  \<sqsubseteq>\<^sub>F\<^sub>D Q \<Longrightarrow> P\<^sup>p\<^sup>r\<^sup>o\<^sup>c\<^sup>+ \<sqsubseteq>\<^sub>F\<^sub>D Q\<close> to  \<longleftrightarrow>\<close>
 
@@ -301,15 +299,24 @@ lemma eat_lemma: \<open>P\<^sup>p\<^sup>r\<^sup>o\<^sup>c\<^sup>* \<sqsubseteq>\
 proof (rule trans_FD)
   show \<open>P\<^sup>p\<^sup>r\<^sup>o\<^sup>c\<^sup>* \<sqsubseteq>\<^sub>F\<^sub>D \<sqinter>a\<in>UNIV \<rightarrow> Q\<close>
     apply (subst GlobalNdet_iterations'_is_Ndet_GlobalNdet_iterations)
-    apply (rule mono_Ndet_FD_right)
-    apply (subst GlobalNdet_iterations_is_one_step_ahead_GlobalNdet_iterations')
-    by (intro mono_Mndetprefix_FD ballI \<open>P\<^sup>p\<^sup>r\<^sup>o\<^sup>c\<^sup>* \<sqsubseteq>\<^sub>F\<^sub>D Q\<close>)
-next
+    by (metis FD_iff_eq_Ndet GlobalNdet_iterations_is_one_step_ahead_GlobalNdet_iterations' Ndet_assoc mono_Mndetprefix_FD that)
+  next
   show \<open>(\<sqinter>a\<in>UNIV \<rightarrow> Q) \<sqsubseteq>\<^sub>F\<^sub>D a \<rightarrow> Q\<close>
     by (simp add: prefix_proving_Mndetprefix_UNIV_ref(3))
 qed
 
-
+lemma eat_read_lemma: 
+  assumes "inj c" "\<And> v. P\<^sup>p\<^sup>r\<^sup>o\<^sup>c\<^sup>* \<sqsubseteq>\<^sub>F\<^sub>D Q v"
+  shows \<open>P\<^sup>p\<^sup>r\<^sup>o\<^sup>c\<^sup>* \<sqsubseteq>\<^sub>F\<^sub>D c\<^bold>?v \<rightarrow> Q v\<close>
+proof (rule trans_FD)
+  show \<open>P\<^sup>p\<^sup>r\<^sup>o\<^sup>c\<^sup>* \<sqsubseteq>\<^sub>F\<^sub>D \<sqinter>a\<in>UNIV \<rightarrow> P\<^sup>p\<^sup>r\<^sup>o\<^sup>c\<^sup>*\<close>
+    by (simp add: Mndetprefix_GlobalNdet eat_lemma mono_GlobalNdet_FD_const)
+next
+  show "\<sqinter>a\<in>UNIV \<rightarrow> P\<^sup>p\<^sup>r\<^sup>o\<^sup>c\<^sup>* \<sqsubseteq>\<^sub>F\<^sub>D (c\<^bold>?v \<rightarrow> Q v)"
+    apply (rule read_proving_Mndetprefix_UNIV_ref)
+      apply (simp_all add: assms)
+    done
+qed
 
 
 lemma iterate_F_imp_GlobalNdet_iterations_F :
@@ -363,7 +370,7 @@ proof -
                 \<open>length t = Suc i\<close> \<open>(u, range ev) \<in> \<F> P\<close> by blast
     from "*"(1, 2, 3) obtain a t'
       where ** : \<open>e = ev a\<close> \<open>t = ev a # t'\<close> \<open>s = t' @ u\<close> \<open>tickFree t'\<close> \<open>length t' = i\<close>
-      by (cases t; simp add: tickFree_def) (use event.exhaust in blast)
+      by (cases t; simp add: tickFree_def) (metis "*"(2) is_ev_def tickFree_Cons_iff)
     hence \<open>(s, range ev) \<in> (\<Union>i. {a. case a of (s, X) \<Rightarrow> tickFree s \<and> length s < Suc i \<and> (\<exists>a. ev a \<notin> X)} \<union>
             {(s @ t, X) |s t X. tickFree s \<and> length s = Suc i \<and> (t, X) \<in> \<F> P})\<close>
       (* TODO: write a better proof *)
@@ -372,40 +379,28 @@ proof -
   qed
   ultimately show \<open>deadlock_free P\<close>
     unfolding AfterExt.deadlock_free_is_right(2)
-    by (metis (no_types, lifting) append_single_T_imp_tickFree is_processT5_S7 subsetD)
+    by (metis (no_types, lifting) front_tickFree_nonempty_append_imp gr0_conv_Suc is_processT2_TR
+        is_processT5_S7 length_0_conv length_Suc_conv less_irrefl subset_iff)
 qed
 
-lemma 
-
-GlobalNdet_iterations_FD_imp_deadlock_free :
+lemma GlobalNdet_iterations_FD_imp_deadlock_free :
   \<open>P\<^sup>p\<^sup>r\<^sup>o\<^sup>c\<^sup>+ \<sqsubseteq>\<^sub>F\<^sub>D P \<Longrightarrow> deadlock_free P\<close>
   by (simp add: GlobalNdet_iterations_F_imp_deadlock_free leFD_imp_leF)
 
-
-text\<open>Benoit 30Jan\<close>
-(* this is already proven in the branch of parameterized termination *)
-lemma GlobalNdet_Seq : \<open>(\<sqinter> a\<in>A. P a) \<^bold>; Q = \<sqinter> a\<in>A. (P a \<^bold>; Q)\<close>
-  apply (cases \<open>A = {}\<close>, simp add: STOP_Seq)
-  apply (simp add: Process_eq_spec F_GlobalNdet D_GlobalNdet T_GlobalNdet F_Seq D_Seq)
-  by safe blast+
-
-lemma Mndetprefix_Seq : \<open>(\<sqinter>a\<in>A \<rightarrow> P a) \<^bold>; Q = \<sqinter>a\<in>A \<rightarrow> (P a \<^bold>; Q)\<close>
-  apply (simp add: Mndetprefix_GlobalNdet GlobalNdet_Seq)
-  apply (rule mono_GlobalNdet_eq)
-  by (simp add: write0_def Mprefix_Seq)
-
 text \<open> York: This would be a useful lemma to have, because it would allow us to have an operator that simply does n event steps. 24Jan25
- proved by Benoit 30Jan\<close>
-lemma iterate_is_iterate_SKIP_Seq :
-  \<open>iterate i\<cdot>(\<Lambda> X. \<sqinter>a\<in>UNIV \<rightarrow> X)\<cdot>P = iterate i\<cdot>(\<Lambda> X. \<sqinter>a\<in>UNIV \<rightarrow> X)\<cdot>SKIP \<^bold>; P\<close>
+ proved by Benoit 30Jan, SKIP to Skip 25Feb\<close>
+lemma iterate_is_iterate_SKIP_Seq :  \<open>iterate i\<cdot>(\<Lambda> X. \<sqinter>a\<in>UNIV \<rightarrow> X)\<cdot>P = iterate i\<cdot>(\<Lambda> X. \<sqinter>a\<in>UNIV \<rightarrow> X)\<cdot>Skip \<^bold>; P\<close>
 proof (induct i)
-  show \<open>iterate 0\<cdot>(\<Lambda> X. \<sqinter>a\<in>UNIV \<rightarrow>  X)\<cdot>P = iterate 0\<cdot>(\<Lambda> X. \<sqinter>a\<in>UNIV \<rightarrow>  X)\<cdot>SKIP \<^bold>; P\<close>
-    by (simp add: SKIP_Seq)
+  show \<open>iterate 0\<cdot>(\<Lambda> X. \<sqinter>a\<in>UNIV \<rightarrow>  X)\<cdot>P =
+        iterate 0\<cdot>(\<Lambda> X. \<sqinter>a\<in>UNIV \<rightarrow>  X)\<cdot>Skip \<^bold>; P\<close> by simp
 next
-  fix i assume hyp : \<open>iterate i\<cdot>(\<Lambda> X. \<sqinter>a\<in>UNIV \<rightarrow>  X)\<cdot>P = iterate i\<cdot>(\<Lambda> X. \<sqinter>a\<in>UNIV \<rightarrow>  X)\<cdot>SKIP \<^bold>; P\<close>
-  show \<open>iterate (Suc i)\<cdot>(\<Lambda> X. \<sqinter>a\<in>UNIV \<rightarrow>  X)\<cdot>P = iterate (Suc i)\<cdot>(\<Lambda> X. \<sqinter>a\<in>UNIV \<rightarrow>  X)\<cdot>SKIP \<^bold>; P\<close>
+  fix i assume hyp : \<open>iterate i\<cdot>(\<Lambda> X. \<sqinter>a\<in>UNIV \<rightarrow> X)\<cdot>P = iterate i\<cdot>(\<Lambda> X. \<sqinter>a\<in>UNIV \<rightarrow>  X)\<cdot>Skip \<^bold>; P\<close>
+  show \<open>iterate (Suc i)\<cdot>(\<Lambda> X. \<sqinter>a\<in>UNIV \<rightarrow>  X)\<cdot>P =
+        iterate (Suc i)\<cdot>(\<Lambda> X. \<sqinter>a\<in>UNIV \<rightarrow>  X)\<cdot>Skip \<^bold>; P\<close>
     by (auto simp add: Mndetprefix_Seq intro: mono_Mndetprefix_eq hyp)
 qed
+
+
 
 
 text\<open>Benoit 30Jan\<close>
@@ -419,17 +414,16 @@ lemma GlobalNdet_iterations'_GlobalNdet_iterations' : \<open>(P\<^sup>p\<^sup>r\
        apply blast
       apply (metis append.assoc tickFree_append_iff)
      apply blast
-    apply (metis eq_Nil_appendI non_tickFree_implies_nonMt)
+     apply (metis append_self_conv2 non_tickFree_imp_not_Nil)
    apply (metis append.assoc tickFree_append_iff)
   using tickFree_Nil by blast
+
 
 text\<open>Benoit 30Jan, the original is lemma \<open>(P\<^sup>p\<^sup>r\<^sup>o\<^sup>c\<^sup>+)\<^sup>p\<^sup>r\<^sup>o\<^sup>c\<^sup>+ = P\<^sup>p\<^sup>r\<^sup>o\<^sup>c\<^sup>+\<close>\<close>
 lemma GlobalNdet_iterations_GlobalNdet_iterations : \<open>(P\<^sup>p\<^sup>r\<^sup>o\<^sup>c\<^sup>+)\<^sup>p\<^sup>r\<^sup>o\<^sup>c\<^sup>+ = \<sqinter>a\<in>UNIV \<rightarrow> P\<^sup>p\<^sup>r\<^sup>o\<^sup>c\<^sup>+\<close>
   by (simp add: GlobalNdet_iterations_is_one_step_ahead_GlobalNdet_iterations'
                 GlobalNdet_iterations'_Mndetprefix
                 GlobalNdet_iterations'_GlobalNdet_iterations')
-
-
 
 
 
@@ -463,7 +457,8 @@ thm prefix_proving_Mndetprefix_UNIV_ref(3)
 text\<open>York 31Jan25:\<close>
 
 lemma no_step_refine: "P\<^sup>p\<^sup>r\<^sup>o\<^sup>c\<^sup>* \<sqsubseteq>\<^sub>F\<^sub>D P"
-  by (simp add: GlobalNdet_iterations'_is_Ndet_GlobalNdet_iterations)
+  by (simp add: GlobalNdet_iterations'_is_Ndet_GlobalNdet_iterations Ndet_FD_self_left)
+
 
 (*
 thm binops_proving_Mndetprefi*
@@ -476,79 +471,102 @@ lemma df_step_intro:
   assumes P_def: "P = Q" "P\<^sup>p\<^sup>r\<^sup>o\<^sup>c\<^sup>+ \<sqsubseteq>\<^sub>F\<^sub>D Q"
   shows "deadlock_free P"
   apply (rule GlobalNdet_iterations_FD_imp_deadlock_free)
-  apply (subst P_def) back
+  apply (subst P_def)  back (* apply (subst (2) P_def) *)
   apply (simp add: assms(2))
   done
 
 lemma ndet_prefix_ext_choice:(*this is added for P = d\<rightarrow>( (a \<rightarrow> b \<rightarrow> P) \<box> (b \<rightarrow> c \<rightarrow> P)) pattern: prefix of external choice*)
   assumes "P\<^sup>p\<^sup>r\<^sup>o\<^sup>c\<^sup>* \<sqsubseteq>\<^sub>F\<^sub>D Q" "P\<^sup>p\<^sup>r\<^sup>o\<^sup>c\<^sup>* \<sqsubseteq>\<^sub>F\<^sub>D R"
   shows "P\<^sup>p\<^sup>r\<^sup>o\<^sup>c\<^sup>* \<sqsubseteq>\<^sub>F\<^sub>D Q \<box> R"
-  by (metis CSP.mono_Det_FD Det_id assms(1) assms(2))
+  by (metis mono_Det_FD Det_id assms(1) assms(2))
 
 
-lemma guard_choice:(*this is added for P =  (a & \<rightarrow> P) \<box> (b \<rightarrow> c \<rightarrow> P) pattern: prefix of external choice*)
-  assumes "P\<^sup>p\<^sup>r\<^sup>o\<^sup>c\<^sup>* \<sqsubseteq>\<^sub>F\<^sub>D a \<^bold>&  Q" "P\<^sup>p\<^sup>r\<^sup>o\<^sup>c\<^sup>* \<sqsubseteq>\<^sub>F\<^sub>D b \<^bold>&  R"
-  shows "P\<^sup>p\<^sup>r\<^sup>o\<^sup>c\<^sup>* \<sqsubseteq>\<^sub>F\<^sub>D a  \<^bold>& Q \<box> b  \<^bold>&  R"
-  by (metis CSP.mono_Det_FD Det_id assms(1) assms(2))
+
+lemma guard_choice:(*this is added for P =  (a & (c\<rightarrow> P)) \<box> (b &  (c \<rightarrow> P)) pattern: prefix of external choice*)
+  assumes "P\<^sup>p\<^sup>r\<^sup>o\<^sup>c\<^sup>* \<sqsubseteq>\<^sub>F\<^sub>D (a \<^bold>&  Q)" "P\<^sup>p\<^sup>r\<^sup>o\<^sup>c\<^sup>* \<sqsubseteq>\<^sub>F\<^sub>D (b \<^bold>&  R)"
+  shows "P\<^sup>p\<^sup>r\<^sup>o\<^sup>c\<^sup>* \<sqsubseteq>\<^sub>F\<^sub>D (a  \<^bold>& Q) \<box> (b  \<^bold>&  R)"
+  by (metis mono_Det_FD Det_id assms(1) assms(2))
 
 
-text\<open>The mothod\<close>
+text\<open>The method\<close>
 method deadlock_free uses P_def =
   (rule df_step_intro[OF P_def],
    simp add: one_step_ahead_GlobalNdet_iterations'_FD_iff_GlobalNdet_iterations_FD[THEN sym],
-   simp add: prefix_proving_Mndetprefix_UNIV_ref(3) eat_lemma no_step_refine binops_proving_Mndetprefix_ref ndet_prefix_ext_choice)
+   simp add: prefix_proving_Mndetprefix_UNIV_ref(3) eat_lemma no_step_refine 
+             binops_proving_Mndetprefix_ref ndet_prefix_ext_choice)
 
 
 text\<open>examples\<close>
-lemma
-  assumes P_def: \<open>P = (a \<rightarrow> b \<rightarrow> c \<rightarrow> d \<rightarrow> P)\<close>
-  shows \<open>deadlock_free P\<close>
-  apply (rule GlobalNdet_iterations_FD_imp_deadlock_free)
-  apply (simp add: one_step_ahead_GlobalNdet_iterations'_FD_iff_GlobalNdet_iterations_FD[THEN sym])
-  apply (subst P_def) back
-  apply (simp add: eat_lemma no_step_refine prefix_proving_Mndetprefix_UNIV_ref(3))
-  done
 
-lemma 
+
+lemma ex1_m:
+  assumes P_def: \<open>P = (a \<rightarrow> b \<rightarrow> c \<rightarrow> d \<rightarrow> P)\<close>
+  shows \<open>deadlock_free P\<close> 
+  apply (rule GlobalNdet_iterations_FD_imp_deadlock_free)
+  apply (subst P_def) back
+  apply (simp add: one_step_ahead_GlobalNdet_iterations'_FD_iff_GlobalNdet_iterations_FD[THEN sym])
+  apply (rule prefix_proving_Mndetprefix_UNIV_ref(3))
+  apply (rule eat_lemma)+
+  apply (rule no_step_refine)
+  done 
+
+lemma ex1_m':
+  assumes P_def: \<open>P = (a \<rightarrow> b \<rightarrow> c \<rightarrow> d \<rightarrow> P)\<close>
+  shows \<open>deadlock_free P\<close> 
+  apply (rule df_step_intro[OF P_def])
+  apply (simp add: one_step_ahead_GlobalNdet_iterations'_FD_iff_GlobalNdet_iterations_FD
+[THEN sym])
+  by (simp add: eat_lemma no_step_refine prefix_proving_Mndetprefix_UNIV_ref(3))(*through sledgehammer*)
+ 
+
+lemma ex1_a:
   assumes P_def: \<open>P = (a \<rightarrow> b \<rightarrow> c \<rightarrow> d \<rightarrow> P)\<close>
   shows \<open>deadlock_free P\<close>
   by (deadlock_free P_def: P_def)
 
-
-
-lemma 
+lemma ex2_m:
   assumes P_def: \<open>P = (a \<rightarrow> b \<rightarrow> P) \<box> (b \<rightarrow> c \<rightarrow> P)\<close>
   shows \<open>deadlock_free P\<close>
   apply (rule GlobalNdet_iterations_FD_imp_deadlock_free)
+  apply (subst (2) P_def)
   apply (simp add: one_step_ahead_GlobalNdet_iterations'_FD_iff_GlobalNdet_iterations_FD[THEN sym])
-  apply (subst P_def) back
-  apply (simp add: binops_proving_Mndetprefix_ref(2) eat_lemma no_step_refine prefix_proving_Mndetprefix_UNIV_ref(3))
+    apply (simp add: binops_proving_Mndetprefix_ref(2) eat_lemma 
+                   no_step_refine prefix_proving_Mndetprefix_UNIV_ref(3) )
   done
 
-lemma 
+lemma ex2_a:
   assumes P_def': \<open>P = (a \<rightarrow> b \<rightarrow> P) \<box> (b \<rightarrow> c \<rightarrow> P)\<close>
   shows \<open>deadlock_free P\<close>
   by (deadlock_free P_def: P_def')
 
-
-
-
-lemma 
+lemma ex3_m:
   assumes P_def: \<open>P = d\<rightarrow>( (a \<rightarrow> b \<rightarrow> P) \<box> (b \<rightarrow> c \<rightarrow> P))\<close>
   shows \<open>deadlock_free P\<close>  
   apply (rule GlobalNdet_iterations_FD_imp_deadlock_free)
+  apply (subst (2) P_def)
   apply (simp add: one_step_ahead_GlobalNdet_iterations'_FD_iff_GlobalNdet_iterations_FD[THEN sym])
-  apply (subst P_def) back
-
-  apply (simp add: eat_lemma ndet_prefix_ext_choice  no_step_refine prefix_proving_Mndetprefix_UNIV_ref(3))
+  apply (rule prefix_proving_Mndetprefix_UNIV_ref(3))
+  apply (rule ndet_prefix_ext_choice)
+   apply (rule eat_lemma)+
+  apply (rule no_step_refine)
+   apply (rule eat_lemma)+
+  apply (rule no_step_refine)
   done
 
-lemma 
+
+lemma ex3_m':
   assumes P_def: \<open>P = d\<rightarrow>( (a \<rightarrow> b \<rightarrow> P) \<box> (b \<rightarrow> c \<rightarrow> P))\<close>
+  shows \<open>deadlock_free P\<close>  
+  apply (rule GlobalNdet_iterations_FD_imp_deadlock_free)
+  apply (subst (2) P_def)
+  apply (simp add: one_step_ahead_GlobalNdet_iterations'_FD_iff_GlobalNdet_iterations_FD[THEN sym])
+  apply (simp add: eat_lemma ndet_prefix_ext_choice  no_step_refine prefix_proving_Mndetprefix_UNIV_ref(3) )
+  done
+
+lemma ex3_a:
+  assumes P_def: \<open>P = e\<rightarrow>( (a \<rightarrow> b \<rightarrow> P) \<box> (b \<rightarrow> c \<rightarrow> P))\<close>
   shows \<open>deadlock_free P\<close>
-  by (deadlock_free P_def: P_def)
-
-
+by (deadlock_free P_def: P_def)
 
 
 
@@ -557,36 +575,86 @@ text\<open>lemmas from 'Bounded_Buffer_211124_ddf_automation_incomplete' by Simo
 lemma Mndetprefix_trans_subset_FD : 
   \<open>A \<noteq> {} \<Longrightarrow> A \<subseteq> B \<Longrightarrow> (\<And>a. a \<in> A \<Longrightarrow> Q a \<sqsubseteq>\<^sub>F\<^sub>D P a) \<Longrightarrow>
    Mndetprefix B Q \<sqsubseteq>\<^sub>F\<^sub>D Mndetprefix A P\<close>
-  by (metis CSP.mono_Mndetprefix_FD mono_Mndetprefix_FD_set trans_FD)
+  by (simp add: prefix_proving_Mndetprefix_ref(1))
 
 lemma Ndet_trans_Det_FD :\<open>P \<sqsubseteq>\<^sub>F\<^sub>D Q \<Longrightarrow> R \<sqsubseteq>\<^sub>F\<^sub>D S \<Longrightarrow> P \<sqinter> R \<sqsubseteq>\<^sub>F\<^sub>D Q \<box> S\<close>
-  by (meson CSP.mono_Ndet_FD mono_Ndet_Det_FD trans_FD)
+  by (meson Ndet_FD_Det dual_order.trans mono_Det_FD)
 
 find_theorems "(\<box>)" "(\<sqsubseteq>\<^sub>F\<^sub>D)"
 
 
-lemma DF_guard_extchoice:
-  assumes "b \<Longrightarrow> DF UNIV \<sqsubseteq>\<^sub>F\<^sub>D Q" "c \<Longrightarrow> DF UNIV \<sqsubseteq>\<^sub>F\<^sub>D R" "b \<or> c"
+lemma DF_guard_extchoice:  assumes "b \<Longrightarrow> DF UNIV \<sqsubseteq>\<^sub>F\<^sub>D Q" "c \<Longrightarrow> DF UNIV \<sqsubseteq>\<^sub>F\<^sub>D R" "b \<or> c"
   shows "DF UNIV \<sqsubseteq>\<^sub>F\<^sub>D (b \<^bold>& Q) \<box> (c \<^bold>& R)"
-  by (metis Det_STOP Det_commute Guard_False Guard_True assms(1) assms(2) assms(3) deadlock_free_Det deadlock_free_def)
+  by (metis (full_types) Det_STOP Det_commute Guard_False Guard_True assms deadlock_free_Det deadlock_free_def)
 
-lemma refine_guarded_extchoice:
-  assumes "b \<or> c" "b \<Longrightarrow> \<sqinter>x\<in>UNIV \<rightarrow> X \<sqsubseteq>\<^sub>F\<^sub>D Q" "c \<Longrightarrow> \<sqinter>x\<in>UNIV \<rightarrow> X \<sqsubseteq>\<^sub>F\<^sub>D R"
+lemma refine_guarded_extchoice:   assumes "b \<or> c" "b \<Longrightarrow> \<sqinter>x\<in>UNIV \<rightarrow> X \<sqsubseteq>\<^sub>F\<^sub>D Q" "c \<Longrightarrow> \<sqinter>x\<in>UNIV \<rightarrow> X \<sqsubseteq>\<^sub>F\<^sub>D R"
   shows "\<sqinter>x\<in>UNIV \<rightarrow>  X \<sqsubseteq>\<^sub>F\<^sub>D (b \<^bold>& Q) \<box> (c \<^bold>& R)"
-  by (metis Det_STOP Det_commute FD_iff_eq_Ndet Guard_def Ndet_trans_Det_FD assms(1) assms(2) assms(3) idem_FD)
+  by (metis Det_STOP Det_commute FD_iff_eq_Ndet Guard_def Ndet_trans_Det_FD assms idem_FD)
 
 lemma extchoice_preguard: "(b \<or> c) \<^bold>& (b \<^bold>& Q) \<box> (c \<^bold>& R) = (b \<^bold>& Q) \<box> (c \<^bold>& R)"
   by (simp add: Guard_def)
 
-lemma MultiDet_preguard: "finite I \<Longrightarrow> (Sup (b ` I) \<^bold>& (\<^bold>\<box> i\<in>I. b i \<^bold>& P i)) = (\<^bold>\<box> i\<in>I. b i \<^bold>& P i)"
-  apply (induct arbitrary: b P rule: finite_induct)
-  apply (auto simp add: Guard_def Det_is_STOP_iff MultiDet_is_STOP_iff)
-  apply (metis Det_id)
-  done
+lemma GlobalDet_is_STOP_iff : \<open>\<box>a \<in> A. P a = STOP \<longleftrightarrow> (\<forall>a \<in> A. P a = STOP)\<close>
+  \<comment>\<open>Missing in the theory\<close>
+  by (simp add: STOP_iff_T T_GlobalDet, safe, auto)
 
-lemma generilized_refine_guarded_extchoice:
-  assumes "finite I" "\<exists>i\<in>I. b(i)" "\<And> i. \<lbrakk> i \<in> I; b(i) \<rbrakk> \<Longrightarrow> \<sqinter>x\<in>UNIV \<rightarrow> X \<sqsubseteq>\<^sub>F\<^sub>D P(i)" 
-  shows "\<sqinter>x\<in>UNIV \<rightarrow> X \<sqsubseteq>\<^sub>F\<^sub>D (\<^bold>\<box> i\<in>I. b(i) \<^bold>& P(i))"
+
+find_theorems \<open>Sup\<close> \<open>?a :: bool set\<close>
+
+lemma MultiDet_preguard: "finite I \<Longrightarrow> (Sup (b ` I) \<^bold>& (\<box> i\<in>I. b (i) \<^bold>& (P i))) = (\<box> i\<in>I. b i \<^bold>& P i)"
+  apply (induct arbitrary: b P rule: finite_induct)
+   apply (auto simp add: Guard_def Det_is_STOP_iff GlobalDet_is_STOP_iff)
+  by (metis (mono_tags, lifting) GlobalDet_factorization_union GlobalDet_unit STOP_Det
+      insert_def singleton_conv)
+
+lemma GlobalDet_preguard :
+  \<comment>\<open>Without the assumption \<^term>\<open>finite I\<close>.\<close>
+  \<open>(Sup (b ` I) \<^bold>& (\<box> i\<in>I. b (i) \<^bold>& (P i))) = \<box> i\<in>I. b i \<^bold>& P i\<close>
+  by (auto intro: Process_eq_optimizedI
+      simp add: Guard_def GlobalDet_projs STOP_projs
+      split: if_split_asm)
+
+lemma GlobalDet_preguard_bis :\<open>\<box>i \<in> I. b i \<^bold>& P i = \<box>i \<in> {i \<in> I. b i}. P i\<close>
+proof -
+  have \<open>{i \<in> I. b i} \<union> {i \<in> I. \<not> b i} = I\<close> by blast
+  hence \<open>\<box> i\<in>I. b i \<^bold>& P i = (\<box>i \<in> {i \<in> I. b i}. b i \<^bold>& P i) \<box> (\<box>i \<in> {i \<in> I. \<not> b i}. b i \<^bold>& P i)\<close>
+    by (simp add: GlobalDet_factorization_union)
+  also have \<open>\<box>i \<in> {i \<in> I. b i}. b i \<^bold>& P i = \<box>i \<in> {i \<in> I. b i}. P i\<close>
+    by (auto intro: mono_GlobalDet_eq)
+  also have \<open>\<box>i \<in> {i \<in> I. \<not> b i}. b i \<^bold>& P i = STOP\<close>
+    by (simp add: GlobalDet_is_STOP_iff)
+  finally show \<open>\<box>i \<in> I. b i \<^bold>& P i = \<box>i \<in> {i \<in> I. b i}. P i\<close> by simp
+qed
+
+
+lemma generalized_refine_guarded_extchoice:
+  assumes (* "finite I" *) \<open>\<exists>i\<in>I. b(i)\<close> \<open>\<And> i. \<lbrakk> i \<in> I; b(i) \<rbrakk> \<Longrightarrow> \<sqinter>a \<in> UNIV \<rightarrow> X \<sqsubseteq>\<^sub>F\<^sub>D P(i)\<close>
+  shows \<open>\<sqinter>a \<in> UNIV \<rightarrow> X \<sqsubseteq>\<^sub>F\<^sub>D \<box> i\<in>I. b(i) \<^bold>& P(i)\<close>
+proof (unfold GlobalDet_preguard_bis)
+  have \<open>\<box>i \<in> {i \<in> I. b i}. \<sqinter>a \<in> UNIV \<rightarrow> X \<sqsubseteq>\<^sub>F\<^sub>D \<box>i \<in> {i \<in> I. b i}. P i\<close>
+    by (auto intro: mono_GlobalDet_FD assms(2))
+  also have \<open>\<box>i \<in> {i \<in> I. b i}. \<sqinter>a \<in> UNIV \<rightarrow> X = \<sqinter>a \<in> UNIV \<rightarrow> X\<close>
+    apply (rule GlobalDet_id)
+    using \<open>\<exists>i\<in>I. b(i)\<close> by blast
+  finally show \<open>\<sqinter>a \<in> UNIV \<rightarrow> X \<sqsubseteq>\<^sub>F\<^sub>D \<box>i \<in> {i \<in> I. b i}. P i\<close> .
+qed
+
+lemma generalized_refine_guarded_extchoice_star:
+  assumes \<open>\<exists>i\<in>I. b(i)\<close> \<open>\<And> i. \<lbrakk> i \<in> I; b(i) \<rbrakk> \<Longrightarrow> \<sqinter>a \<in> UNIV \<rightarrow> X\<^sup>p\<^sup>r\<^sup>o\<^sup>c\<^sup>* \<sqsubseteq>\<^sub>F\<^sub>D P(i)\<close>
+  shows \<open>X\<^sup>p\<^sup>r\<^sup>o\<^sup>c\<^sup>* \<sqsubseteq>\<^sub>F\<^sub>D \<box> i\<in>I. b(i) \<^bold>& P(i)\<close>
+proof (rule trans_FD)
+  show \<open>X\<^sup>p\<^sup>r\<^sup>o\<^sup>c\<^sup>* \<sqsubseteq>\<^sub>F\<^sub>D \<sqinter>a\<in>UNIV \<rightarrow> X\<^sup>p\<^sup>r\<^sup>o\<^sup>c\<^sup>*\<close>
+    by (simp add: Mndetprefix_GlobalNdet eat_lemma mono_GlobalNdet_FD_const)
+next
+  show "\<sqinter>a\<in>UNIV \<rightarrow> X\<^sup>p\<^sup>r\<^sup>o\<^sup>c\<^sup>* \<sqsubseteq>\<^sub>F\<^sub>D \<box>i\<in>I. b i \<^bold>& P i"
+    apply (rule generalized_refine_guarded_extchoice)
+    apply (simp_all add: assms)
+    done
+qed
+
+
+text\<open>because we have this pattern on the rhs of the lemma above, we need to normalize the model to match the rhs pattern.\<close>
+(* old proof
 using assms proof (induct arbitrary:X rule:finite_induct)
   case empty
   then show ?case
@@ -595,69 +663,534 @@ next
   case (insert x F)
   then show ?case
   proof -
-    from insert have 1:"(\<^bold>\<box> i\<in>{x} \<union> F. b i \<^bold>& P i) = (b x \<^bold>& P x) \<box> (Sup (b ` F) \<^bold>& (\<^bold>\<box> i\<in>F. b i \<^bold>& P i))"
-      by (smt (verit, ccfv_threshold) Guard_def MultiDet_insert' MultiDet_is_STOP_iff Sup_bool_def True_in_image_Bex insert_is_Un)
-    have 2:"\<sqinter>x\<in>UNIV \<rightarrow> X \<sqsubseteq>\<^sub>F\<^sub>D (b x \<^bold>& P x) \<box> (Sup (b ` F) \<^bold>& (\<^bold>\<box> i\<in>F. b i \<^bold>& P i))"
+    from insert have 1:"(\<box> i\<in>({x} \<union> F). b i \<^bold>& P i) = (b x \<^bold>& P x) \<box> (Sup (b ` F) \<^bold>& (\<box> i\<in>F. b i \<^bold>& P i))"
+      sledgehammer
+      by (smt (verit, ccfv_threshold) Guard_def GlobalDet_insert' MultiDet_is_STOP_iff Sup_bool_def True_in_image_Bex insert_is_Un)
+    have 2:"\<sqinter>x\<in>UNIV \<rightarrow> X \<sqsubseteq>\<^sub>F\<^sub>D (b x \<^bold>& P x) \<box> (Sup (b ` F) \<^bold>& (\<box> i\<in>F. b i \<^bold>& P i))"
       apply (rule refine_guarded_extchoice, auto simp add: Sup_bool_def insert)
       using Sup_bool_def insert.prems(1) apply blast
       done
     thus ?thesis
       using "1" by fastforce
   qed
-qed
+qed *)
 
 
-text\<open>Examples\<close>
-lemma (*is this deadlock free?*)
-  assumes P_def: \<open>P = ((x < 0) \<^bold>& (a \<rightarrow> P)) \<box>(( x \<ge> 0) \<^bold>& (b \<rightarrow> P))\<close>
+lemma ex4_m:
+  assumes P_def: \<open>P = ((x<(0::int)) \<^bold>& (a \<rightarrow> P)) \<box>(( x \<ge> 0) \<^bold>& (b \<rightarrow> P))\<close>
+  shows \<open>deadlock_free P\<close>
+  apply (rule df_step_intro[OF P_def])
+  apply (simp add: one_step_ahead_GlobalNdet_iterations'_FD_iff_GlobalNdet_iterations_FD[THEN sym])
+  apply (rule refine_guarded_extchoice)
+  apply auto
+  apply (rule prefix_proving_Mndetprefix_UNIV_ref)
+  apply (rule no_step_refine)  
+  apply (rule prefix_proving_Mndetprefix_UNIV_ref)
+  apply (rule no_step_refine)
+  done
+
+lemma ex4_m':
+  assumes P_def: \<open>P = ((x<(0::int)) \<^bold>& (a \<rightarrow> P)) \<box>(( x \<ge> 0) \<^bold>& (b \<rightarrow> P))\<close>
+  shows \<open>deadlock_free P\<close>
+  apply (rule df_step_intro[OF P_def])
+  apply (simp add: one_step_ahead_GlobalNdet_iterations'_FD_iff_GlobalNdet_iterations_FD[THEN sym])
+  apply (simp add: Guard_def no_step_refine prefix_proving_Mndetprefix_UNIV_ref(3) refine_guarded_extchoice)
+  done
+
+
+lemma ex4_m'':
+  assumes P_def: \<open>P = ((x<(0::int)) \<^bold>& (a \<rightarrow> P)) \<box>(( x \<ge> 0) \<^bold>& (b \<rightarrow> P))\<close>
+  shows \<open>deadlock_free P\<close>
+  apply (rule df_step_intro[OF P_def])
+  by (simp add: GlobalNdet_iterations_is_one_step_ahead_GlobalNdet_iterations' 
+                Guard_def no_step_refine prefix_proving_Mndetprefix_UNIV_ref(3))
+ (*also work using 
+  by (auto intro!: refine_guarded_extchoice prefix_proving_Mndetprefix_UNIV_ref no_step_refine 
+         simp add: one_step_ahead_GlobalNdet_iterations'_FD_iff_GlobalNdet_iterations_FD[THEN sym])
+ *)
+  
+
+
+method deadlock_free_guard uses P_def =
+  (rule df_step_intro[OF P_def]
+  , simp add: one_step_ahead_GlobalNdet_iterations'_FD_iff_GlobalNdet_iterations_FD[THEN sym]
+  prefix_proving_Mndetprefix_UNIV_ref(3) eat_lemma no_step_refine 
+             binops_proving_Mndetprefix_ref ndet_prefix_ext_choice Guard_def )
+(*refine_guarded_extchoice not needed*)
+(*does not work if change the 2nd simp into auto intro!,  why? ? *)
+
+method deadlock_free_guard'' uses P_def =
+  (rule df_step_intro[OF P_def]
+  ,auto intro!: eat_lemma refine_guarded_extchoice 
+                prefix_proving_Mndetprefix_UNIV_ref no_step_refine  
+simp add: one_step_ahead_GlobalNdet_iterations'_FD_iff_GlobalNdet_iterations_FD[THEN sym])
+(*does not work for all examples, so not useful*)
+
+
+lemma ex1_a':
+  assumes P_def: \<open>P = (a \<rightarrow> b \<rightarrow> c \<rightarrow> d \<rightarrow> P)\<close>
+  shows \<open>deadlock_free P\<close>
+  by (deadlock_free_guard P_def: P_def)
+
+
+lemma ex2_a':
+  assumes P_def': \<open>P = (a \<rightarrow> b \<rightarrow> P) \<box> (b \<rightarrow> c \<rightarrow> P)\<close>
+  shows \<open>deadlock_free P\<close>
+  by (deadlock_free_guard P_def: P_def')
+
+
+lemma ex3_a':
+  assumes P_def: \<open>P = d\<rightarrow>( (a \<rightarrow> b \<rightarrow> P) \<box> (b \<rightarrow> c \<rightarrow> P))\<close>
+  shows \<open>deadlock_free P\<close>
+by (deadlock_free_guard P_def: P_def)
+
+
+lemma ex4_auto:
+  assumes P_def: \<open>P = (x < (0::int)) \<^bold>& (a \<rightarrow> P) \<box>( x \<ge> 0) \<^bold>& (b \<rightarrow> P)\<close>
+  shows \<open>deadlock_free P\<close>
+  by (deadlock_free_guard P_def: P_def)
+
+
+
+lemma ex5:
+  assumes P_def: \<open>P = e\<rightarrow>((x < (0::int)) \<^bold>& (a \<rightarrow> P)) \<box>(( x \<ge> 0) \<^bold>& (b \<rightarrow> P))\<close>
   shows \<open>deadlock_free P\<close>
   apply (rule GlobalNdet_iterations_FD_imp_deadlock_free)
   apply (simp add: one_step_ahead_GlobalNdet_iterations'_FD_iff_GlobalNdet_iterations_FD[THEN sym])
-  apply (subst P_def) back
+  apply (subst (2) P_def)
+  by (simp add: Guard_def eat_lemma no_step_refine prefix_proving_Mndetprefix_UNIV_ref(3))
 
-  oops
-
-lemma 
-  assumes P_def: \<open>P = e\<rightarrow>(((x < 0) \<^bold>& (a \<rightarrow> P)) \<box>(( x \<ge> 0) \<^bold>& (b \<rightarrow> P)))\<close>
+lemma ex5_a:
+  assumes P_def: \<open>P = e\<rightarrow>((x < (0::int)) \<^bold>& (a \<rightarrow> P)) \<box>(( x \<ge> 0) \<^bold>& (b \<rightarrow> P))\<close>
   shows \<open>deadlock_free P\<close>
-
-  oops
-
+  by (deadlock_free_guard P_def: P_def)
 
 
-lemma 
-  assumes P_def: \<open>P =( b \<^bold>& P \<box> c \<^bold>& Q)\<close>
-  shows \<open>deadlock_free P\<close> 
-  apply (rule GlobalNdet_iterations_FD_imp_deadlock_free)
-  apply (simp add: one_step_ahead_GlobalNdet_iterations'_FD_iff_GlobalNdet_iterations_FD[THEN sym])
-  apply (subst P_def) back
-  oops
+text\<open>guard extchoice generalization\<close>
 
-
-
-
-lemma 
-  assumes P_def: \<open>P = \<^bold>\<box> i\<in>{0,1,2}. if i = 0 then b \<^bold>& P else if i = 1 then c \<^bold>& Q else d \<^bold>& R\<close>
-  shows \<open>deadlock_free P\<close>
-  oops
-
-
-
-lemma 
-  assumes P_def: \<open>P = ((x < 0) \<^bold>& a \<rightarrow> P) \<box>(( x \<ge> 0) \<^bold>& b \<rightarrow> P)\<close>
-  shows \<open>deadlock_free P\<close>
-  by (deadlock_free P_def: P_def)
 
 term "b \<^bold>& P \<box> c \<^bold>& Q"
 
-term "\<^bold>\<box> i\<in>{0,1}. if i = 0 then b \<^bold>& P else c \<^bold>& Q"
+term "b \<^bold>& P "
+term "\<box> i\<in>{0,1::int}. (if i = 0 then b \<^bold>& P else c \<^bold>& Q)"
 
-lemma "\<^bold>\<box> i\<in>{0,1}. if i = 0 then P else Q = P \<box> Q"
-  apply simp
+lemma "\<box> i\<in>{0,1::nat}. (if i = 0 then P else Q) = P \<box> Q"
+  by (simp add: GlobalDet_distrib_unit_bis)
+
+
+lemma bi_extchoice_norm:
+"b \<^bold>& P \<box> c \<^bold>& Q = \<box> i\<in>{0..1::nat}. (if i = 0 then b else c) \<^bold>&(if i = 0 then P else Q)"
+  apply (simp add: GlobalDet_distrib_unit_bis)
+  by (smt (verit, ccfv_threshold) Det_commute GlobalDet_factorization_union GlobalDet_unit 
+        atLeast0_atMost_Suc atLeastAtMost_singleton insert_is_Un
+      old.nat.distinct(1))
+
+
+(*insert for set*)
+find_theorems GlobalDet insert
+term GlobalDet
+lemma "(\<box> i\<in>insert a A. P i) = (P a \<box> (\<box> i\<in>A. P i))"
+  by (metis GlobalDet_factorization_union GlobalDet_unit insert_is_Un)
+
+thm GlobalDet_distrib_unit_bis
+
+thm GlobalDet_distrib_unit
+
+(* not used
+lemma generalized_bi_extchoice_norm':
+"\<box> i\<in>{n::nat..n+1}. (if i = n then b(n) else c) \<^bold>& (if i = n then P(n) else Q) = b(n) \<^bold>& P(n) \<box> c \<^bold>& Q"
+  proof (induction n)
+  case 0
+  then show ?case
+    using bi_extchoice_norm' by auto 
+next
+  case (Suc n)
+  then show ?case 
+     proof -
+       have step1: "\<box> i\<in>{Suc n::nat..Suc n+1}. (if i = Suc n then b(Suc n) else c) \<^bold>&(if i = Suc n then P(Suc n) else Q)
+= \<box> i\<in>{n+1..n+2}. (if i = n+1 then b(n+1) else c) \<^bold>&(if i = n+1 then P(n+1) else Q) "
+         by (metis (no_types, lifting) add.commute add_2_eq_Suc' mono_GlobalDet_eq plus_1_eq_Suc)
+    
+  have IH: "\<box> i\<in>{n::nat..n+1}. (if i = n then b(n) else c) \<^bold>&(if i = n then P(n) else Q) = b(n) \<^bold>& P(n) \<box> c \<^bold>& Q"
+    using Suc.IH .
+
+  also have step2: "\<box> i\<in>{Suc n..Suc n+1}. (if i = Suc n then b(Suc n) else c) \<^bold>&(if i = Suc n then P(Suc n) else Q) 
+= \<box> i\<in>{n+1..n+2}. (if i = n+1 then b(n+1) else c) \<^bold>&(if i = n+1 then P(n+1) else Q)"
+    using step1 by blast
+  
+  have step3: "\<box> i\<in>{n+1..n+2}. (if i = n+1 then b(n+1) else c) \<^bold>&(if i = n+1 then P(n+1) else Q)
+=  \<box> i\<in>{n+1..(n+1)+1}. (if i = n+1 then b(n+1) else c) \<^bold>&(if i = n+1 then P(n+1) else Q)
+"    using Suc_eq_plus1 add_2_eq_Suc' by presburger
+  
+  
+  define m where  " m = n + 1"
+   then have step5: " \<box> i\<in>{n+1..(n+1)+1}. (if i = n+1 then b(n+1) else c) \<^bold>&(if i = n+1 then P(n+1) else Q) 
+= \<box> i\<in>{m..m+1}. (if i = m then b(m) else c) \<^bold>&(if i = m then P(m) else Q) "
+     by blast
+    have step6: "\<box> i\<in>{m..m+1}. (if i = m then b(m) else c) \<^bold>&(if i = m then P(m) else Q) = b(m) \<^bold>& P(m) \<box> c \<^bold>& Q"
+      using IH  
+      
+      oops*)
+
+
+lemma 
+  assumes "\<And> i. i \<in> A \<Longrightarrow> P i = Q i"
+  shows "(\<box>i\<in>A. P i) = (\<box>i\<in>A. Q i)"
+  using assms mono_GlobalDet_eq by blast
+
+text\<open>to push an binary operator term\<open>(\<box>)\<close> into generalized extchoice, this proof does not use induction \<close>
+lemma biextchoic_normalization:
+  "(\<box> i\<in>{0..n::nat}. b(i) \<^bold>& P(i)) \<box> c \<^bold>& Q 
+   = (\<box> i\<in>{0..n+1}. (if i \<le> n then b(i) else c) \<^bold>& (if i \<le> n then P(i) else Q))"
+ (is "?lhs = ?rhs")
+proof -
+  have 1:"{0..Suc n} = insert (Suc n) {0..n}"
+    by (simp add: atLeast0_atMost_Suc)
+  have "?rhs = 
+        c \<^bold>& Q \<box> (\<box>i\<in>{0..n}. (if i \<le> n then b i else c) \<^bold>& (if i \<le> n then P i else Q))"
+    by (simp add: 1 GlobalDet_distrib_unit)
+  also have "... = (\<box>i\<in>{0..n}. (if i \<le> n then b i else c) \<^bold>& (if i \<le> n then P i else Q)) \<box> c \<^bold>& Q"
+    by (meson Det_commute)
+  also have "... = (\<box>i\<in>{0..n}. (b i) \<^bold>& (P i)) \<box> c \<^bold>& Q"
+  proof -
+    have "(\<box>i\<in>{0..n}. (if i \<le> n then b i else c) \<^bold>& (if i \<le> n then P i else Q)) = (\<box>i\<in>{0..n}. (b i) \<^bold>& (P i))"
+      by (rule mono_GlobalDet_eq, simp)
+    thus ?thesis by simp
+  qed
+  finally show ?thesis ..
+qed
+
+
+lemma biextchoic_normalization_rev:
+  "(\<box> i\<in>{0..n::nat}. b(i) \<^bold>& P(i)) \<box> c \<^bold>& Q 
+   = (\<box> i\<in>{0..n+1}. (if i \<le> n then b(i) else c) \<^bold>& (if i \<le> n then P(i) else Q))"
+  apply (rule biextchoic_normalization)
+  done
+
+text\<open>for P that has no guard (i.e., guard = True)\<close>
+lemma biextchoic_normalization_nguard:
+  "(\<box> i\<in>{0..n::nat}. b(i) \<^bold>& P(i)) \<box> Q 
+   = (\<box> i\<in>{0..n+1}. (if i \<le> n then b(i) else True) \<^bold>& (if i \<le> n then P(i) else Q))"
+  (is "?lhs = ?rhs")
+proof -
+  have "?lhs = (\<box> i\<in>{0..n::nat}. b(i) \<^bold>& P(i)) \<box> True \<^bold>& Q"
+    by (simp add: Guard_True)
+  also have "... = ?rhs"
+    using biextchoic_normalization by blast
+  finally show ?thesis .
+qed
+
+lemma biextchoic_normalization_nguard_prefix:
+  "(\<box> i\<in>{0..n::nat}. b(i) \<^bold>& P(i)) \<box> (a \<rightarrow> Q) 
+   = (\<box> i\<in>{0..n+1}. (if i \<le> n then b(i) else True) \<^bold>& (if i \<le> n then P(i) else a \<rightarrow> Q))"
+  (is "?lhs = ?rhs")
+  using biextchoic_normalization_nguard by blast
+
+find_theorems GlobalDet Guard
+
+
+(*
+(*binary \<box>  normalization*)
+lemma biextchoic_normalization:
+"(\<box> i\<in>{0..n::nat}. b(i) \<^bold>& P(i)) \<box> c \<^bold>& Q 
+       = (\<box> i\<in>{0..n+1}. (if i \<le> n then b(i) else c) \<^bold>& (if i \<le> n then P(i) else Q))"
+(is \<open>?lhs n = ?rhs n\<close>)
+proof (induction n)
+  case 0
+  then show ?case 
+    apply auto
+    apply (simp add:bi_extchoice_norm'[THEN sym])
+    by (smt (verit, best) mono_GlobalDet_eq)
+next
+  (*case (Suc n)
+  then show ?case *)
+  fix n
+  assume hyp: "(\<box> i\<in>{0..n::nat}. b(i) \<^bold>& P(i)) \<box> c \<^bold>& Q 
+       = (\<box> i\<in>{0..n+1}. (if i \<le> n then b(i) else c) \<^bold>& (if i \<le> n then P(i) else Q))"
+     proof -
+    have step1: "(\<box>  i\<in>{0..Suc n}. b(i)  \<^bold>&  P(i))\<box> c \<^bold>& Q 
+                 = (\<box> i\<in>{0..n}. b(i) \<^bold>&  P(i)) \<box> (b(Suc n) \<^bold>&  P(Suc n)) \<box> (c \<^bold>& Q) "
+      by (simp add: Det_commute GlobalDet_distrib_unit_bis atLeast0AtMost atMost_Suc)
+    also have step2: "... = (\<box> i\<in>{0..n}. b(i) \<^bold>&  P(i))  \<box> (c \<^bold>& Q) \<box> (b(Suc n) \<^bold>&  P(Suc n))"
+      by (metis (full_types) Det_assoc Det_commute)
+
+    also have step3: "(\<box> i\<in>{0..(Suc n +1)}. (if i \<le> (Suc n) then b(i) else c) \<^bold>& (if i \<le> (Suc n) then P(i) else Q))
+                      =  (\<box> i\<in>{0..(Suc n + 1)}. (if i \<le> n then b(i) else (if i= Suc n then b(Suc n) else c))
+                                              \<^bold>& (if i \<le> n then P(i) else (if i=Suc n then P(Suc n) else  Q)))  "
+      by (smt (verit, best) le_Suc_eq mono_GlobalDet_eq)
+    also have 
+    oops
+    
+  then show ?thesis sorry
+qed 
+*)
+
+
+
+term "\<box> i\<in>I. b(i) \<^bold>& P(i)"
+
+
+
+
+
+lemma ex7: 
+  assumes P_def: \<open>P = \<box> i\<in>{0..2::nat}. b(i) \<^bold>& (a\<rightarrow> P)\<close> and 
+   \<open> \<exists>i\<in>{0..2}. b i  \<close>
+  shows\<open>deadlock_free (P) \<close>
+ apply (rule df_step_intro[OF P_def])
+  apply (simp add: one_step_ahead_GlobalNdet_iterations'_FD_iff_GlobalNdet_iterations_FD[THEN sym]
+  prefix_proving_Mndetprefix_UNIV_ref(3) eat_lemma no_step_refine 
+             binops_proving_Mndetprefix_ref ndet_prefix_ext_choice)
+  apply (rule generalized_refine_guarded_extchoice)
+  using assms apply auto[1] 
+  apply (simp add: no_step_refine prefix_proving_Mndetprefix_UNIV_ref(3))
+  done
+
+
+lemma ex7': 
+  assumes 
+    P_def: \<open>\<And> i. P i = (\<box> i\<in>{0..3::nat}. b(i) \<^bold>& (a \<rightarrow> P i))\<close>  and
+    prp: \<open>b(0::nat) \<or> b(1) \<or> b(2) \<or> b(3) \<close>
+  shows\<open>deadlock_free (P x)\<close>
+  apply (rule df_step_intro[OF P_def])
+  apply (simp add: one_step_ahead_GlobalNdet_iterations'_FD_iff_GlobalNdet_iterations_FD[THEN sym]
+  prefix_proving_Mndetprefix_UNIV_ref(3) eat_lemma no_step_refine 
+             binops_proving_Mndetprefix_ref ndet_prefix_ext_choice)
+  thm generalized_refine_guarded_extchoice
+  apply (rule generalized_refine_guarded_extchoice)
+  using assms apply auto[1]
+  thm assms
+  apply (rule no_step_refine prefix_proving_Mndetprefix_UNIV_ref(3))
+  by (metis P_def no_step_refine )
+
+
+
+lemma ex7'': 
+  assumes 
+    P_def: \<open>\<And> i. P i = (\<box> i\<in>{0..3::nat}. b(i) \<^bold>& (a \<rightarrow> P i))\<close> 
+  shows\<open>b(0::nat) \<or> b(1) \<or> b(2) \<or> b(3) \<Longrightarrow> deadlock_free (P x)\<close>
+  apply (rule df_step_intro[OF P_def])
+  apply (simp add: one_step_ahead_GlobalNdet_iterations'_FD_iff_GlobalNdet_iterations_FD[THEN sym]
+  prefix_proving_Mndetprefix_UNIV_ref(3) eat_lemma no_step_refine 
+             binops_proving_Mndetprefix_ref ndet_prefix_ext_choice)
+  thm generalized_refine_guarded_extchoice
+  apply (rule generalized_refine_guarded_extchoice)
+  apply auto[1]
+  apply (rule no_step_refine prefix_proving_Mndetprefix_UNIV_ref(3) )
+  by (metis assms no_step_refine)
+
+
+ 
+
+
+lemma ex8: 
+  assumes P_def: \<open>P = b(0) \<^bold>& (a \<rightarrow> P) \<box> b(1) \<^bold>& (a\<rightarrow>P) \<box> b(2) \<^bold>& (a \<rightarrow>P)\<close>and
+   prp: \<open>b(0::nat) \<or> b(1) \<or> b(2)  \<close>
+ shows\<open>deadlock_free P \<close>
+  (* Apply induction *)
+  apply (rule df_step_intro[OF P_def])
+  (* Normalisation *)
+  apply (simp add: biextchoic_normalization bi_extchoice_norm)
+  (* Rewrite the goal to allow multiple events *)
+  apply (simp add: one_step_ahead_GlobalNdet_iterations'_FD_iff_GlobalNdet_iterations_FD[THEN sym])
+  (* Introduction for generalised external choice *)
+  apply (rule generalized_refine_guarded_extchoice)
+  (* Sledgehammer the guard disjunction *)
+  using prp
+  apply (metis One_nat_def Suc_n_not_le_n atMost_atLeast0 atMost_iff le0 le_Suc_eq)
+  (* Simplify away the remaining events *)
+  by (simp add: no_step_refine prefix_proving_Mndetprefix_UNIV_ref(3))
+  
+(*this is not a correct format*)
+lemma ex9: 
+  assumes P_def: \<open> P =  b(0) \<^bold>& ((a\<rightarrow>Skip)\<^bold>;(a\<rightarrow> P0) ) \<box>  b(1) \<^bold>& ((c\<rightarrow>Skip)\<^bold>;(a\<rightarrow> P1)) \<box> b(2) \<^bold>& (a \<rightarrow>P2) \<close> and 
+   \<open>b(0::nat) \<or> b(1)  \<or> b(2)   \<close>
+ shows\<open>deadlock_free( P ) \<close>
+  apply (rule df_step_intro[OF P_def])
+  apply (simp add: biextchoic_normalization bi_extchoice_norm read_Seq write_Seq write0_Seq)
+  apply (simp add: one_step_ahead_GlobalNdet_iterations'_FD_iff_GlobalNdet_iterations_FD[THEN sym])
+  apply (rule generalized_refine_guarded_extchoice)
+  using assms(2) atLeast0AtMost apply auto[1]
+  thm generalized_refine_guarded_extchoice
+ 
   oops
 
+ find_theorems SKIP 
 
-term "\<^bold>\<box> i\<in>I. b(i) \<^bold>& P(i)"
+
+(*Do we need extra lemmas for Skip? or is this deadlock?*)
+lemma "deadlock_free Skip"
+  oops
+
+lemma ex_Skip:
+  assumes P_def:" P = terminate \<rightarrow> Skip" 
+  shows\<open>deadlock_free P \<close>
+  apply (rule GlobalNdet_iterations_FD_imp_deadlock_free)  
+  apply (subst P_def)  back 
+apply (simp add: one_step_ahead_GlobalNdet_iterations'_FD_iff_GlobalNdet_iterations_FD[THEN sym])
+  apply (rule prefix_proving_Mndetprefix_UNIV_ref(3))
+
+  thm Seq_SKIP
+  oops 
+
+lemma ex10: 
+  assumes P_def: \<open>\<And> i. P i  =  e \<rightarrow> (b(0) \<^bold>& ((a\<rightarrow>Skip)\<^bold>;(a\<rightarrow> P(0)) )\<box>  b(1) \<^bold>& ((c\<rightarrow>Skip)\<^bold>;(a\<rightarrow> P(1))) \<box> (terminate \<rightarrow> P(3)) )\<close> and 
+   \<open>b(0::nat) \<or> b(1)   \<close>
+  shows\<open>deadlock_free (P x) \<close>
+   (* Apply induction *)
+  apply (rule df_step_intro[OF P_def])
+  (* Normalisation for the extchoice and seq*)
+  apply (simp add: biextchoic_normalization bi_extchoice_norm biextchoic_normalization_nguard read_Seq write_Seq write0_Seq)
+  (* Rewrite the goal to allow multiple events *)
+  apply (simp add: one_step_ahead_GlobalNdet_iterations'_FD_iff_GlobalNdet_iterations_FD[THEN sym] )
+  apply (rule prefix_proving_Mndetprefix_UNIV_ref(3))
+  thm generalized_refine_guarded_extchoice
+  (* Introduction for generalised external choice *)
+  apply (rule generalized_refine_guarded_extchoice_star)
+   (* Sledgehammer the guard disjunction *)
+  using atLeast0AtMost apply auto[1]
+  thm prefix_proving_Mndetprefix_UNIV_ref(3)
+  (* Simplify away the remaining events *)
+  apply simp
+  by (metis P_def eat_lemma no_step_refine prefix_proving_Mndetprefix_UNIV_ref(3))
+
+lemma "deadlock_free (\<sqinter> x\<in>UNIV. P x) \<Longrightarrow> deadlock_free (P a)"
+  by (simp add: deadlock_free_GlobalNdet_iff)
 
 
+lemma ex11: 
+  assumes P_def: \<open>\<And> i. P i  =  e \<rightarrow> (b(0) \<^bold>& ((a\<rightarrow>Skip)\<^bold>;(a\<rightarrow> P (0)) ) \<box>  b(1) \<^bold>& ((c\<rightarrow>Skip)\<^bold>;(a\<rightarrow> P(1))) \<box>  b(2) \<^bold>& ((d\<rightarrow>Skip)\<^bold>;(a\<rightarrow> P(2))) \<box> (terminate \<rightarrow> P(3)) )\<close> and 
+   \<open>b(0::nat) \<or> b(1)  \<or> b(2)  \<close>
+  shows\<open>deadlock_free (P x) \<close>
+   (* Apply induction *)
+  apply (rule df_step_intro[OF P_def])
+  (* Normalisation for the extchoice and seq*)
+
+(* apply (simp add: bi_extchoice_norm  biextchoic_normalization  biextchoic_normalization_nguard_prefix read_Seq write_Seq write0_Seq) this will fail to push b2 into bi, as Isaelle will apply biextchoic_normalization_nguard before biextchoic_normalization.
+the correct application order of the lemmas
+  apply (simp add: bi_extchoice_norm  )
+  apply (simp add: biextchoic_normalization  )
+  apply (simp add: biextchoic_normalization_nguard  )
+*)
+  apply (simp add: bi_extchoice_norm  biextchoic_normalization  biextchoic_normalization_nguard_prefix read_Seq write_Seq write0_Seq)
+  (* Rewrite the goal to allow multiple events *)
+  apply (simp add: one_step_ahead_GlobalNdet_iterations'_FD_iff_GlobalNdet_iterations_FD[THEN sym] )
+  apply (rule prefix_proving_Mndetprefix_UNIV_ref(3))
+
+  (* Introduction for generalised external choice *)
+  apply (rule generalized_refine_guarded_extchoice_star)
+   (* Sledgehammer the guard disjunction *)
+  using atLeast0AtMost apply auto[1]
+
+(*why is 
+
+  by (simp add: P_def eat_lemma no_step_refine prefix_proving_Mndetprefix_UNIV_ref(3))
+not working here while works in  ex11_step2_df_m ?
+try with new laptop*)
+  apply auto
+  by (metis P_def eat_lemma no_step_refine prefix_proving_Mndetprefix_UNIV_ref(3))+
+
+text\<open>with ex11, now the task is to use auto intro to apply refinement rules instead of using metis. because we need to integrate this into proof method, and metis can not be used in a proof method. \<close>
+
+
+text\<open>The method for normalization: to remove as many operators as possible, this version covers guard, extchoice and sequence\<close>
+method normalization uses P_def =
+  (subst P_def
+  , simp add: bi_extchoice_norm  biextchoic_normalization  biextchoic_normalization_nguard_prefix read_Seq write_Seq write0_Seq)
+
+
+
+lemma ex11_step1_norm_manul:
+  assumes P_def: \<open>\<And> i. P i  =  e \<rightarrow> (b(0) \<^bold>& ((a\<rightarrow>Skip)\<^bold>;(a\<rightarrow> P (0)) ) \<box>  b(1) \<^bold>& ((c\<rightarrow>Skip)\<^bold>;(a\<rightarrow> P(1))) \<box>  b(2) \<^bold>& ((d\<rightarrow>Skip)\<^bold>;(a\<rightarrow> P(2))) \<box> (terminate \<rightarrow> P(3)) )\<close>
+
+shows \<open> (P x)  = e \<rightarrow>
+    \<box>i\<in>{0..Suc (Suc (Suc 0))}.
+       (if i \<le> Suc (Suc 0) then if i \<le> Suc 0 then if i = 0 then b 0 else b (Suc 0) else b 2 else True) \<^bold>&
+       (if i \<le> Suc (Suc 0) then if i \<le> Suc 0 then if i = 0 then a \<rightarrow> a \<rightarrow> P 0 else c \<rightarrow> a \<rightarrow> P 1 else d \<rightarrow> a \<rightarrow> P 2
+        else terminate \<rightarrow> P 3) \<close>
+  apply (subst P_def)
+  apply (simp add: bi_extchoice_norm  biextchoic_normalization  biextchoic_normalization_nguard_prefix read_Seq write_Seq write0_Seq)
+  done
+
+
+lemma ex11_step1_norm_auto:
+  assumes P_def: \<open>\<And> i. P i  =  e \<rightarrow> (b(0) \<^bold>& ((a\<rightarrow>Skip)\<^bold>;(a\<rightarrow> P (0)) ) \<box>  b(1) \<^bold>& ((c\<rightarrow>Skip)\<^bold>;(a\<rightarrow> P(1))) \<box>  b(2) \<^bold>& ((d\<rightarrow>Skip)\<^bold>;(a\<rightarrow> P(2))) \<box> (terminate \<rightarrow> P(3)) )\<close>
+
+shows \<open> (P x)  = e \<rightarrow>
+    \<box>i\<in>{0..Suc (Suc (Suc 0))}.
+       (if i \<le> Suc (Suc 0) then if i \<le> Suc 0 then if i = 0 then b 0 else b (Suc 0) else b 2 else True) \<^bold>&
+       (if i \<le> Suc (Suc 0) then if i \<le> Suc 0 then if i = 0 then a \<rightarrow> a \<rightarrow> P 0 else c \<rightarrow> a \<rightarrow> P 1 else d \<rightarrow> a \<rightarrow> P 2
+        else terminate \<rightarrow> P 3) \<close>
+  by (normalization P_def: P_def)
+ 
+
+
+lemma ex11_step2_df_m: 
+  assumes P_def: \<open>\<And> i. P i  = e \<rightarrow>
+    \<box>i\<in>{0..Suc (Suc (Suc 0))}.
+       (if i \<le> Suc (Suc 0) then if i \<le> Suc 0 then if i = 0 then b 0 else b (Suc 0) else b 2 else True) \<^bold>&
+       (if i \<le> Suc (Suc 0) then if i \<le> Suc 0 then if i = 0 then a \<rightarrow> a \<rightarrow> P 0 else c \<rightarrow> a \<rightarrow> P 1 else d \<rightarrow> a \<rightarrow> P 2
+        else terminate \<rightarrow> P 3)\<close> and 
+   \<open>b(0::nat) \<or> b(1)  \<or> b(2)  \<close>
+ shows\<open>deadlock_free (P x) \<close>
+  apply (rule df_step_intro[OF P_def])
+ (* Rewrite the goal to allow multiple events *)
+  apply (simp add: one_step_ahead_GlobalNdet_iterations'_FD_iff_GlobalNdet_iterations_FD[THEN sym] )
+  apply (rule prefix_proving_Mndetprefix_UNIV_ref(3))
+  thm assms
+  (* Introduction for generalised external choice *)
+  apply (rule generalized_refine_guarded_extchoice_star)
+   (* Sledgehammer the guard disjunction *)
+  using atLeast0AtMost apply auto[1]
+  by (simp add: P_def eat_lemma no_step_refine prefix_proving_Mndetprefix_UNIV_ref(3))
+
+
+
+text\<open>The method for deadlock freedom after normalization\<close>
+method deadlock_free_normed uses P_def assms=
+  (rule df_step_intro[OF P_def]
+  , simp add: one_step_ahead_GlobalNdet_iterations'_FD_iff_GlobalNdet_iterations_FD[THEN sym]
+, rule prefix_proving_Mndetprefix_UNIV_ref(3)
+, rule generalized_refine_guarded_extchoice_star
+, insert atLeast0AtMost assms, auto
+, auto intro!: P_def eat_lemma no_step_refine prefix_proving_Mndetprefix_UNIV_ref(3))
+
+lemma ex11_step2_df_a: 
+  assumes P_def: \<open>\<And> i. P i  = e \<rightarrow>
+    \<box>i\<in>{0..Suc (Suc (Suc 0))}.
+       (if i \<le> Suc (Suc 0) then if i \<le> Suc 0 then if i = 0 then b 0 else b (Suc 0) else b 2 else True) \<^bold>&
+       (if i \<le> Suc (Suc 0) then if i \<le> Suc 0 then if i = 0 then a \<rightarrow> a \<rightarrow> P 0 else c \<rightarrow> a \<rightarrow> P 1 else d \<rightarrow> a \<rightarrow> P 2
+        else terminate \<rightarrow> P 3)\<close> and 
+   \<open>b(0::nat) \<or> b(1)  \<or> b(2)  \<close>
+ shows\<open>deadlock_free (P x) \<close>
+  by (deadlock_free_normed P_def: P_def)
+
+
+
+
+
+
+lemma ex11_no_para:
+  assumes P_def: \<open>P =  e \<rightarrow> (b(0) \<^bold>& ((a\<rightarrow>Skip)\<^bold>;(a\<rightarrow> P) ) \<box>  b(1) \<^bold>& ((c\<rightarrow>Skip)\<^bold>;(a\<rightarrow> P)) \<box>  b(2) \<^bold>& ((d\<rightarrow>Skip)\<^bold>;(a\<rightarrow> P)) \<box> (terminate \<rightarrow> P) )\<close> and 
+   \<open>b(0::nat) \<or> b(1)  \<or> b(2)  \<close>
+  shows\<open>deadlock_free P \<close>
+   (* Apply induction *)
+  apply (rule df_step_intro[OF P_def])
+  (* Normalisation for the extchoice and seq*)
+  apply (simp add: biextchoic_normalization bi_extchoice_norm biextchoic_normalization_nguard_prefix read_Seq write_Seq write0_Seq)
+ (*? ? ? b2 is not discharged*)
+
+  (* Rewrite the goal to allow multiple events *)
+  apply (simp add: one_step_ahead_GlobalNdet_iterations'_FD_iff_GlobalNdet_iterations_FD[THEN sym] )
+
+  (* Apply refinement laws to discharge the goal *)
+  apply (auto intro!:prefix_proving_Mndetprefix_UNIV_ref(3) generalized_refine_guarded_extchoice_star eat_lemma no_step_refine)
+  done  
+
+
+lemma ex12: 
+  assumes P_def: \<open>\<And> i. P i  =  e \<rightarrow> (b(0) \<^bold>& ((a\<rightarrow>Skip)\<^bold>;(a\<rightarrow> P(0)) ) \<box>  b(1) \<^bold>& ((c\<rightarrow>Skip)\<^bold>;(a\<rightarrow> P(1))) \<box>  b(2) \<^bold>& ((d\<rightarrow>Skip)\<^bold>;(a\<rightarrow> P(2))) \<box> (terminate \<rightarrow> Skip) )\<close> and 
+   \<open>b(0::nat) \<or> b(1)  \<or> b(2)  \<close>
+ shows\<open>deadlock_free (P x) \<close>
+  oops
 end
