RingBuffer/Guard-old.thy
@@ -1,10 +1,10 @@
 
-theory "Guard"
+theory Guard
   imports "HOL-CSP_OpSem.Operational_Semantics_Laws"
 begin
 
 
-definition Guard :: \<open>bool \<Rightarrow> ('a, 'r) process\<^sub>p\<^sub>t\<^sub>i\<^sub>c\<^sub>k \<Rightarrow> ('a, 'r) process\<^sub>p\<^sub>t\<^sub>i\<^sub>c\<^sub>k \<close> (infixl \<open>\<^bold>&\<close> 84)
+definition Guard :: \<open>bool \<Rightarrow> 'e process \<Rightarrow> 'e process\<close> (infixl \<open>\<^bold>&\<close> 81)
   where \<open>b \<^bold>& P \<equiv> if b then P else STOP\<close>
 
 lemma Guard_cont [simp] : \<open>cont P \<Longrightarrow> cont (\<lambda>x. b \<^bold>& P x)\<close>
@@ -21,11 +21,11 @@ lemma Guard_STOP [simp] : \<open>b \<^bold>& STOP = STOP\<close>
   by (simp add: Guard_def)
 
 
-lemma Guard_Ndet : \<open>b \<^bold>& (P \<sqinter> Q) = b \<^bold>& P \<sqinter> b \<^bold>& Q\<close>
-  by (simp add: Guard_def)
+lemma Guard_Ndet : \<open>b \<^bold>& (P \<sqinter> Q) =( b \<^bold>& P) \<sqinter> (b \<^bold>& Q)\<close>
+  by (simp add: Guard_def Ndet_id)
 
-lemma Guard_Det : \<open>b \<^bold>& (P \<box> Q) = b \<^bold>& P \<box> b \<^bold>& Q\<close>
-  by (simp add: Guard_def)
+lemma Guard_Det : \<open>b \<^bold>& (P \<box> Q) = (b \<^bold>& P) \<box> (b \<^bold>& Q)\<close>
+  by (simp add: Guard_def Det_id)
 
 (* 
 lemma Det_Guard : \<open>(b \<^bold>& P) \<box> Q = (if b then P \<box> Q else Q)\<close>
@@ -37,43 +37,41 @@ lemma Guard_Sliding : \<open>b \<^bold>& (P \<rhd> Q) = b \<^bold>& P \<rhd> b \
   by (simp add: Guard_def Sliding_id)
 
 lemma Guard_Seq : \<open>b \<^bold>& (P \<^bold>; Q) = b \<^bold>& P \<^bold>; b \<^bold>& Q\<close>
-  by (simp add: Guard_def)
+  by (simp add: Guard_def STOP_Seq)
 
 lemma Guard_Sync : \<open>b \<^bold>& (P \<lbrakk>S\<rbrakk> Q) = b \<^bold>& P \<lbrakk>S\<rbrakk> b \<^bold>& Q\<close>
   by (simp add: Guard_def)
 
 
-lemma Guard_Mprefix : \<open>b \<^bold>& (\<box>a\<in>A \<rightarrow> P a) = \<box>a\<in>{a. a \<in> A \<and> b} \<rightarrow> P a\<close>
+lemma Guard_Mprefix : \<open>b \<^bold>& (\<box>a\<in>A \<rightarrow> P a) = (\<box>a\<in>{a. a \<in> A \<and> b} \<rightarrow> P a)\<close>
   by (simp add: Guard_def )
 
-lemma Guard_Mndetprefix : \<open>b \<^bold>& (\<sqinter>a\<in>A \<rightarrow> P a) = \<sqinter>a\<in>{a. a \<in> A \<and> b} \<rightarrow> P a\<close>
+lemma Guard_Mndetprefix : \<open>b \<^bold>& (\<sqinter>a\<in>A \<rightarrow> P a) = (\<sqinter>a\<in>{a. a \<in> A \<and> b} \<rightarrow> P a)\<close>
   by (simp add: Guard_def )
 
 
-lemma Guard_Interrupt : \<open>b \<^bold>& (P \<triangle> Q) = b \<^bold>& P \<triangle> b \<^bold>& Q\<close>
+lemma Guard_Interrupt : \<open>b \<^bold>& (P \<triangle> Q) = (b \<^bold>& P) \<triangle> (b \<^bold>& Q)\<close>
   by (simp add: Guard_def )
 
 
 lemma Guard_Throw : \<open>b \<^bold>& (P \<Theta> a\<in>A. Q a) = b \<^bold>& P \<Theta> a\<in>A. b \<^bold>& Q a\<close>
-  by (simp add: Guard_def)
+  by (simp add: Guard_def Throw_STOP)
 
 lemma Guard_Hiding : \<open>b \<^bold>& (P \ S) = b \<^bold>& P \ S\<close>
   by (simp add: Guard_def )
 
-lemma Guard_Renaming : \<open>b \<^bold>& Renaming P f g = Renaming (b \<^bold>& P) f g\<close>
-  by (simp add: Guard_def)
+lemma Guard_Renaming : \<open>b \<^bold>& Renaming P f = Renaming (b \<^bold>& P) f\<close>
+  by (simp add: Guard_def )
 
 
 lemma initials_Guard : \<open>(b \<^bold>& P)\<^sup>0 = (if b then P\<^sup>0 else {})\<close>
-  by (simp add: Guard_def)
+  by (simp add: Guard_def initials_STOP)
 
 
-lemma (in After) After_Guard : \<open>(b \<^bold>& P) after a = (if b then P after a else \<Psi> STOP a)\<close>
+lemma (in After) After_Guard : \<open>b \<^bold>& P after e = (if b then P after e else \<Psi> STOP e)\<close>
   by (simp add : Guard_def After_STOP)
 
-lemma (in AfterExt) After_Guard :
-  \<open>(b \<^bold>& P) after\<^sub>\<checkmark> e = (  if b then P after\<^sub>\<checkmark> e
-                       else case e of ev a \<Rightarrow> \<Psi> STOP a | \<checkmark>(r) \<Rightarrow> \<Omega> STOP r)\<close>
+lemma (in AfterExt) After_Guard : \<open>b \<^bold>& P after\<^sub>\<checkmark> e = (if b then P after\<^sub>\<checkmark> e else case e of ev x \<Rightarrow> \<Psi> STOP x | \<checkmark> \<Rightarrow> \<Omega> STOP)\<close>
   by (simp add: After\<^sub>t\<^sub>i\<^sub>c\<^sub>k_STOP Guard_def)
 
 lemma (in OpSemTransitions) \<tau>_trans_Guard :
